making progress 11 with new type

semantics/programs.v
@@ -181,7 +181,7 @@ Inductive trace_i1: iconf -> iconf -> obseq -> the_write_stuff -> Prop :=
     trace_c (N, V, c) (N1, V1, c1) O W ->
     checkpoint \notin O ->
     trace_i1 (Cc, N, V, c) (Cc, N1, V1, c1) O W
-  iTrace_RB: forall{N0 N Nrb Nend: nvmem} {V Vmid Vend: vmem} {c cmid cend: command}
+ | iTrace_RB: forall{N0 N Nmid Nend: nvmem} {V Vmid Vend: vmem} {c cstart cmid cend: command}
                  {O1 O2: obseq} {W1 W2: the_write_stuff},
     trace_c (N, V, cstart) (Nmid, Vmid, cmid) O1 W1 -> (*first section of trace w
                                                        no reboots*)
@@ -190,33 +190,32 @@ Inductive trace_i1: iconf -> iconf -> obseq -> the_write_stuff -> Prop :=
     checkpoint \notin O1 ->
     checkpoint \notin O2 ->
     trace_i1 ((N0, V, c), N, V, cstart) ((N0, V, c), Nend, Vend, cend)
-             (O1 ++ [reboot] ++ O2)
+             (O1 ++ [::reboot] ++ O2)
              (append_write W1 W2)
-    iTrace_CP: trace_i1 ((Nc0, Vc0, cc0), N0, V0, c0) ((Nc0, Vc0, cc0), Nmid, Vmid,
-                                                               (inscheckpoint w);;crem) O1 W1 (*1st
+ | iTrace_CP: forall{Nc0 N0 Nmid Nc1 Nend: nvmem} {Vc0 V0 Vmid Vc1 Vend: vmem}
+                         {cc0 c0 crem cc1 cend: command}
+                         {O1 O2: obseq} {W1 W2: the_write_stuff}
+      {w: warvars},
+      trace_i1 ((Nc0, Vc0, cc0), N0, V0, c0) ((Nc0, Vc0, cc0), Nmid, Vmid,
+                                                               (incheckpoint w);;crem) O1 W1 (*1st
                                                                                                checkpointed section*)
                         -> checkpoint \notin O1
                         -> trace_i1 (((Nc0 |! w), Vmid, crem), Nmid, Vmid, crem)
                                    ((Nc1, Vc1, cc1), Nend, Vend, cend) O2 W2
                         -> trace_i1 ((Nc0, Vc0, cc0), N0, V0, c0)
                                    ((Nc1, Vc1, cc1), Nend, Vend, cend)
-                                   O1 ++ [checkpoint] ++ O2
-                                  (append_write W1 W2).
+                                   (O1 ++ [::checkpoint] ++ O2)
+                                   (append_write W1 W2).
+
+
 (*cant define it in terms of continuous (actually you can if you
 prove it equivalent to other def)
  *)
-.
-(*cons to the front*)
-|iTrace_Single: forall{C1 C2: iconf} {O: obseq} {W: the_write_stuff},
-                  iceval_w C1 O C2 W -> (*command in C2 is skip by def single_com, iceval_w*)
-                  trace_i C1 C2 O W
-| iTrace_App: forall{C1 C2 Cmid: iconf} {O1 O2: obseq}
-         {W1 W2: the_write_stuff},
-    trace_i C1 Cmid O1 W1 -> (*steps first section*)
-    trace_i Cmid C2 O2 W2 -> (*steps rest of program*)
-    O1 <> [::] -> (* forces empty step to use other constructors*)
-    O2 <> [::]  ->
-    trace_i C1 C2 (O1 ++ O2) (append_write W1 W2).
+Theorem trace_convert: forall{C1 C2: iconf} {O: obseq} {W: the_write_stuff},
+    trace_i C1 C2 O W <-> trace_i1 C1 C2 O W.
+Admitted.
+
+
 
 Open Scope nat_scope.
 
@@ -286,7 +285,7 @@ Definition FstWt {C1 C2: context} {O: obseq} {W: the_write_stuff}
  V1 isn't used anywhere it's just to fill out the type
  N2, V2 is final state for intermittent, once again solely to fill out the type*)
 
-Inductive same_pt: nvmem -> vmem -> command -> command -> nvmem -> vmem -> nvmem -> Prop:=
+Inductive same_pt: nvmem -> vmem -> command -> command -> nvmem -> nvmem -> Prop:=
 same_mem: forall {N0 N1 Ncomp N2: nvmem}
                   {V0 V1 V2: vmem}
                   {c0 c1 crem: command}
@@ -301,7 +300,7 @@ same_mem: forall {N0 N1 Ncomp N2: nvmem}
                  -> (forall(l: loc),
                       not((getmap N1) l = (getmap Ncomp) l)
                       -> ((l \in (getwt W2)) /\ (l \in (getfstwt (append_write W1 W2))) /\ not (l \in (getwt W1))))
-                  -> same_pt N0 V0 c0 c1 N1 V1 Ncomp.
+                  -> same_pt N0 V0 c0 c1 N1(*V1*) Ncomp.
 (*Definition 5*)
 (*Nc0 is starting nvm for cont
 Ni0 is starting nvm for intermittent
@@ -324,7 +323,7 @@ Inductive current_init_pt: nvmem -> vmem -> command -> nvmem -> nvmem -> nvmem -
                  -> (forall(l: loc),
                       not((getmap N1) l = (getmap Nc0) l)
                       -> (l \in (getfstwt W)) \/ (l \in (getdomain N)))
-                 -> current_init_pt N V c Ni0 Nc0.
+                 -> current_init_pt N V c Ni0 N1 (*V1*) Nc0.
 (*Definition 6*)
 (*concern: Typo in paper, N0, V0 is left out of invocation of Def 4*)
 (*(N0, V0, c0) is checkpoint state at time c1
@@ -338,7 +337,7 @@ Inductive same_config: iconf -> context -> Prop :=
   SameConfig: forall(N0 N1 N2: nvmem)
                 (V0 V: vmem)
                 (c0 c: command),
-                same_pt (N0 U! N1) V0 c0 c N1 N2 -> (*nvms are extensionally the same by same_pt
+                same_pt (N0 U! N1) V0 c0 c N1 (*V*) N2 -> (*nvms are extensionally the same by same_pt
                                           vms and cs are intensionally the same by types*)
                 same_config ((N0, V0, c0), N1, V, c) (N2, V, c).
 
